Première version du fby. Vérifier la traduction !!

DataflowListSemantics.v
@@ -4,10 +4,31 @@ Require Import Rustre.Common.
 Require Import Rustre.DataflowSyntax.
 
 
+Definition alls {A B} (v : B) (l : list A) := List.map (fun _ => v) l.
+
+Fixpoint map2 {A B C} (f : A -> B -> C) l1 l2 :=
+  match l1, l2 with
+    | nil, _ => nil
+    | _, nil => nil
+    | x1 :: l1, x2 :: l2 => f x1 x2 :: map2 f l1 l2
+  end.
+
+Lemma map2_nil {A B C} : forall (f : A -> B -> C) l1 l2, map2 f l1 l2 = nil <-> l1 = nil \/ l2 = nil.
+Proof. intros f [| x1 l1] [| x2 l2]; simpl; try tauto. intuition discriminate. Qed.
+
+Lemma map2_cons {A B C} : forall (f : A -> B -> C) l1 l2 y l, map2 f l1 l2 = y :: l <->
+  exists x1 l1' x2 l2', l1 = x1 :: l1' /\ l2 = x2 :: l2' /\ y = f x1 x2 /\ map2 f l1' l2' = l.
+Proof.
+intros f [| x1 l1] [| x2 l2] y l; simpl; split; intro Heq; decompose [and ex] Heq; try now discriminate.
+- inversion Heq. subst. repeat eexists; repeat split; eassumption.
+- subst. inversion_clear H; inversion_clear H0 (* FIXME: generated names *). reflexivity.
+Qed.
+
+
 (** *  Dataflow semantics with lists  **)
 
-(* Idea?: clocks -> instantaneous semantics
-          expressions -> list semantics *)
+(* Idea?: clocks, expressions -> instantaneous semantics
+          equations -> list semantics *)
 Inductive value :=
   | abs
   | here (v : const).
@@ -16,218 +37,192 @@ Coercion here : const >-> value.
 Definition venv := PositiveMap.t value.
 Definition history := list venv.
 
-Definition alls {A B} (v : B) (l : list A) := List.map (fun _ => v) l.
 
+Definition instant_sem_var env x c := PositiveMap.find x env = Some (here c).
 
 Definition sem_var (H : history) (x : ident) (cl : list value) : Prop :=
   List.map (PositiveMap.find x) H = List.map (@Some _) cl.
 
-(** **  Clock semantics  **)
+(** **  Semantics for one instant  **)
 
-(** ***  Clock semantics for one instant  **)
+(** ***  Clock semantics  **)
 
 Inductive instant_sem_clock (env : venv) : clock -> bool -> Prop :=
-| base: instant_sem_clock env Cbase true
-| on_tick:
-    forall ck x b,
+  | base: instant_sem_clock env Cbase true
+  | on_tick: forall ck x b,
       instant_sem_clock env ck true ->
       PositiveMap.find x env = Some (here (Cbool b)) -> 
       instant_sem_clock env (Con ck x b) true
-| on_abs1:
-    forall ck x b,
+  | on_abs1 : forall ck x b,
       instant_sem_clock env ck false ->
       instant_sem_clock env (Con ck x b) false
-| on_abs2:
-    forall ck x c c',
+  | on_abs2 : forall ck x c c',
       instant_sem_clock env ck true ->
       PositiveMap.find x env = Some (here c') -> 
       Cbool c <> c' ->
       instant_sem_clock env (Con ck x c) false.
 
-(** ***  Lifting to lists  **)
+(** ***  Expression semantics  **)
+
+Inductive instant_sem_laexp (env : venv) : laexp -> value -> Prop :=
+  | Stick : forall ck ce c,
+      instant_sem_lexp env ce c ->
+      instant_sem_clock env ck true ->
+      instant_sem_laexp env (LAexp ck ce) c
+  | Sabs : forall ck ce,
+      instant_sem_lexp env ce abs ->
+      instant_sem_clock env ck false ->
+      instant_sem_laexp env (LAexp ck ce) abs
+
+with instant_sem_lexp (env : venv) : lexp -> value -> Prop :=
+  | Sconst : forall c, instant_sem_lexp env (Econst c) c
+  | Svar : forall x c,
+      instant_sem_var env x c ->
+      instant_sem_lexp env (Evar x) c
+  | Swhen_eq : forall s x b c,
+      instant_sem_var env x  (Cbool b) ->
+      instant_sem_laexp env s c ->
+      instant_sem_lexp env (Ewhen s x b) c
+  | Swhen_abs : forall s x b b',
+      instant_sem_var env x (Cbool b') -> b <> b' ->
+      instant_sem_lexp env (Ewhen s x b) abs.
+
+Inductive instant_sem_caexp (env : venv) : caexp -> value -> Prop :=
+  | SCtick : forall ck ce c,
+      instant_sem_cexp env ce c ->
+      instant_sem_clock env ck true ->
+      instant_sem_caexp env (CAexp ck ce) c
+  | SCabs : forall ck ce,
+      instant_sem_cexp env ce abs ->
+      instant_sem_clock env ck false ->
+      instant_sem_caexp env (CAexp ck ce) abs
+
+with instant_sem_cexp (env : venv) : cexp -> value -> Prop :=
+  | Smerge_true : forall x t f c,
+      instant_sem_var env x (Cbool true) ->
+      instant_sem_caexp env t c ->
+      instant_sem_cexp env (Emerge x t f) c
+  | Smerge_false : forall x t f c,
+      instant_sem_var env x (Cbool false) ->
+      instant_sem_caexp env f c ->
+      instant_sem_cexp env (Emerge x t f) c
+  | Sexp : forall e c,
+      instant_sem_lexp env e c ->
+      instant_sem_cexp env (Eexp e) c.
+
+(** **  Lifting to lists  **)
 
 Inductive sem_clock : history -> clock -> list bool -> Prop :=
-  | Snil : forall ck, sem_clock nil ck nil
-  | Scons : forall env H ck b bl, 
+  | Snil_ck : forall ck, sem_clock nil ck nil
+  | Scons_ck : forall env H ck b bl, 
       instant_sem_clock env ck b -> sem_clock H ck bl -> sem_clock (env :: H) ck (b :: bl).
 
-Inductive sem_laexp (H : history) : laexp -> value -> Prop :=
-  | Stick : forall ck ce c,
-      sem_lexp H ce c ->
-      sem_clock H ck true ->
-      sem_laexp H (LAexp ck ce) (here c)
-  | Sabs : forall ck ce,
-      sem_lexp H ce None ->
-      sem_clock H ck false ->
-      sem_laexp H (LAexp ck ce) None
+Inductive sem_laexp : history -> laexp -> list value -> Prop :=
+  | Snil_laexp : forall cae, sem_laexp nil cae nil
+  | Scons_laexp : forall env H cae c cl,
+      instant_sem_laexp env cae c -> sem_laexp H cae cl -> sem_laexp (env :: H) cae (c :: cl).
 
-with sem_lexp (H: history): lexp -> value -> Prop :=
-| Sconst: 
-    forall c n,
-      sem_lexp H (Econst c) n (Some c)
-| Svar: 
-    forall x c n,
-      sem_var H x n c ->
-      sem_lexp H (Evar x) n (Some c)
-| Swhen_eq:
-    forall s x b n c,
-      sem_var H x n  (Cbool b) ->
-      sem_laexp H s n c ->
-      sem_lexp H (Ewhen s x b) n c
-| Swhen_abs:
-    forall s x b b' n,
-      sem_var H x n (Cbool b') ->
-      ~ (b = b') ->
-      sem_lexp H (Ewhen s x b) n None.
-               
+Inductive sem_lexp : history -> lexp -> list value -> Prop :=
+  | Snil_lexp : forall ce, sem_lexp nil ce nil
+  | Scons_lexp : forall env H ce c cl,
+      instant_sem_lexp env ce c -> sem_lexp H ce cl -> sem_lexp (env :: H) ce (c :: cl).
 
-Inductive sem_caexp (H: history): caexp -> nat -> value -> Prop :=
-| SCtick:
-    forall ck ce n c,
-      sem_cexp H ce n (Some c) ->
-      sem_clock H ck n true ->
-      sem_caexp H (CAexp ck ce) n (Some c)
-| SCabs:
-    forall ck ce n,
-      sem_cexp H ce n None ->
-      sem_clock H ck n false ->
-      sem_caexp H (CAexp ck ce) n None
-with sem_cexp (H: history): cexp -> nat -> option const -> Prop :=
-| Smerge_true:
-    forall x t f n c,
-      sem_var H x n (Cbool true) ->
-      sem_caexp H t n c ->
-      sem_cexp H (Emerge x t f) n c
-| Smerge_false:
-    forall x t f n c,
-      sem_var H x n (Cbool false) ->
-      sem_caexp H f n c ->
-      sem_cexp H (Emerge x t f) n c
-| Sexp:
-    forall e n c,
-      sem_lexp H e n c ->
-      sem_cexp H (Eexp e) n c.
+Inductive sem_caexp : history -> caexp -> list value -> Prop :=
+  | Snil_caexp : forall cae, sem_caexp nil cae nil
+  | Scons_caexp : forall env H cae c cl,
+      instant_sem_caexp env cae c -> sem_caexp H cae cl -> sem_caexp (env :: H) cae (c :: cl).
 
-Inductive sem_equation (G: global): history -> equation -> Prop :=
-| SEqDef:
-    forall H x cae,
-      (forall n, 
-       exists v, sem_lexp H (Evar x) n v
-              /\ sem_caexp H cae n v) ->
+Inductive sem_cexp : history -> cexp -> list value -> Prop :=
+  | Snil_cexp : forall cae, sem_cexp nil cae nil
+  | Scons_cexp : forall env H ce c cl,
+      instant_sem_cexp env ce c -> sem_cexp H ce cl -> sem_cexp (env :: H) ce (c :: cl).
+
+
+(** Alternative definition by a forall on lists *)
+Fixpoint for_all2 {A B} (P : A -> B -> Prop) l1 l2 :=
+  match l1, l2 with
+    | nil, nil => True
+    | x1 :: l1, x2 :: l2 => P x1 x2 /\ for_all2 P l1 l2
+    | _ :: _, nil => False
+    | nil, _ :: _ => False
+  end.
+
+Lemma for_all2_length {A B} : forall (P : A -> B -> Prop) l1 l2, for_all2 P l1 l2 -> length l1 = length l2.
+Proof.
+intros P l1. induction l1 as [| x1 l1]; intros l2 Hall.
+- destruct l2; trivial. now elim Hall.
+- destruct l2; try now elim Hall. simpl in *. f_equal. now apply IHl1.
+Qed.
+
+Definition sem_clock' : history -> clock -> list bool -> Prop :=
+  fun H ck bl => for_all2 (fun env => instant_sem_clock env ck) H bl.
+
+Definition sem_laexp' : history -> laexp -> list value -> Prop :=
+  fun H cae cl => for_all2 (fun env => instant_sem_laexp env cae) H cl.
+
+Definition sem_lexp' : history -> lexp -> list value -> Prop :=
+  fun H ce cl => for_all2 (fun env => instant_sem_lexp env ce) H cl.
+
+Definition sem_caexp' : history -> caexp -> list value -> Prop :=
+  fun H cae cl => for_all2 (fun env => instant_sem_caexp env cae) H cl.
+
+Definition sem_cexp' : history -> cexp -> list value -> Prop :=
+  fun H ce cl => for_all2 (fun env => instant_sem_cexp env ce) H cl.
+
+(** Equivalence of both definitions *)
+
+Ltac solve_equiv :=
+  intro H; induction H as [| env H IHH]; intros cae bl;
+  [ split; intro Hsem;
+    [ inversion_clear Hsem; exact I
+    | apply for_all2_length in Hsem; destruct bl; constructor || discriminate ]
+  | split; intro Hsem;
+    [ inversion_clear Hsem; rewrite IHH in *; now split
+    | assert (Hnil : bl <> nil) by (intro; subst; apply for_all2_length in Hsem; discriminate);
+      destruct bl as [| b bl]; try (now elim Hnil); [];
+      destruct Hsem; constructor; trivial; now rewrite IHH ] ].
+
+Lemma sem_clock_equiv : forall H ck bl, sem_clock H ck bl <-> sem_clock' H ck bl.
+Proof. solve_equiv. Qed.
+
+Lemma sem_laexp_equiv : forall H cae cl, sem_laexp H cae cl <-> sem_laexp' H cae cl.
+Proof. solve_equiv. Qed.
+
+Lemma sem_lexp_equiv : forall H cae cl, sem_lexp H cae cl <-> sem_lexp' H cae cl.
+Proof. solve_equiv. Qed.
+
+Lemma sem_caexp_equiv : forall H cae cl, sem_caexp H cae cl <-> sem_caexp' H cae cl.
+Proof. solve_equiv. Qed.
+
+Lemma sem_cexp_equiv : forall H cae cl, sem_cexp H cae cl <-> sem_cexp' H cae cl.
+Proof. solve_equiv. Qed.
+
+
+(** **  Semantics of equations  **)
+
+(** Now we need ot take into account the fby operator.
+    Version of the paper: head of the list = first instant. *)
+Fixpoint fby (v : const) (s : list value) : list value :=
+  match s with
+  | here v' :: s => here v :: fby v' s
+  | abs :: s => abs :: fby v s
+  | nil => nil
+  end.
+
+(* Maybe we should transform "(exists ...) -> ..." into "forall (... -> ...)" *)
+Inductive sem_equation (G : global) : history -> equation -> Prop :=
+  | SEqDef : forall H x cae,
+      (exists v, sem_lexp H (Evar x) v /\ sem_caexp H cae v) ->
       sem_equation G H (EqDef x cae)
-| SEqApp:
-    forall H x f arg input output eqs,
+  | SEqApp : forall H x f arg input output eqs, (* I did not check this one *)
       PositiveMap.find f G = Some (mk_node f input output eqs) ->
-      (exists H' vi vo,
-         forall n, sem_laexp H arg n vi
-                /\ sem_lexp H (Evar x) n vo
-                /\ sem_lexp H' (Evar input.(v_name)) n vi
-                /\ sem_lexp H' (Evar output.(v_name)) n vo
-                /\ List.Forall (sem_equation G H') eqs) ->
-    sem_equation G H (EqApp x f arg).
-
-
-
-
-
-
-
-Definition sem_var env x c := PositiveMap.find x env = Some (here c).
-Check Con. Print const.
-Inductive Lsem_clock (env : Lvenv) : clock -> bool -> Prop :=
-| Lbase: Lsem_clock env Cbase true
-| Lon_tick:
-    forall ck x b,
-      Lsem_clock env ck true ->
-      Lsem_var env x (Cbool b) -> 
-      Lsem_clock env (Con ck x b) true
-| Lon_abs1:
-    forall ck x b,
-      Lsem_clock env ck false ->
-      Lsem_clock env (Con ck x b) false
-| Lon_abs2:
-    forall ck x c c',
-      Lsem_clock env ck true ->
-      Lsem_var env x c' -> 
-      Cbool c <> c' ->
-      Lsem_clock env (Con ck x c) false.
-
-Inductive Lsem_laexp (env : Lvenv) : laexp -> Lvalue -> Prop :=
-| Ltick :
-    forall ck ce c,
-      Lsem_lexp env ce (here c) ->
-      Lsem_clock env ck true ->
-      Lsem_laexp env (LAexp ck ce) c
-| Labs :
-    forall ck ce,
-      Lsem_lexp env ce abs ->
-      Lsem_clock env ck false ->
-      Lsem_laexp env (LAexp ck ce) abs
-
-with Lsem_lexp (env : Lvenv) : lexp -> Lvalue -> Prop :=
-| Lconst : 
-    forall c,
-      Lsem_lexp env (Econst c) (here c)
-| Lvar :
-    forall x c,
-      PositiveMap.find x env = Some c ->
-      Lsem_lexp env (Evar x) c
-| Lwhen_eq :
-    forall s x b c,
-      Lsem_var env x (Cbool b) ->
-      Lsem_laexp env s c ->
-      Lsem_lexp env (Ewhen s x b) c
-| Lwhen_abs :
-    forall s x b b',
-      Lsem_var env x (Cbool b') ->
-      b <> b' ->
-      Lsem_lexp env (Ewhen s x b) abs.
-
-Inductive Lsem_caexp (env : Lvenv) : caexp -> Lvalue -> Prop :=
-| LCtick:
-    forall ck ce c,
-      Lsem_cexp env ce (here c) ->
-      Lsem_clock env ck true ->
-      Lsem_caexp env (CAexp ck ce) (here c)
-| LCabs:
-    forall ck ce,
-      Lsem_cexp env ce abs ->
-      Lsem_clock env ck false ->
-      Lsem_caexp env (CAexp ck ce) abs
-with Lsem_cexp (env: Lvenv) : cexp -> Lvalue -> Prop :=
-| Lmerge_true:
-    forall x t f c,
-      Lsem_var env x (Cbool true) ->
-      Lsem_caexp env t c ->
-      Lsem_cexp env (Emerge x t f) c
-| Lmerge_false:
-    forall x t f c,
-      Lsem_var env x (Cbool false) ->
-      Lsem_caexp env t c ->
-      Lsem_cexp env (Emerge x t f) c
-| Lexp:
-    forall e c,
-      Lsem_lexp env e c ->
-      Lsem_cexp env (Eexp e) c.
-
-Inductive Lsem_equation (env: Lvenv) : equation -> Prop :=
-| LEqDef:
-    forall x cae,
-      (exists v, Lsem_lexp env (Evar x) v
-              /\ Lsem_caexp env cae v) ->
-      Lsem_equation env (EqDef x cae)
-| LEqApp:
-    forall x f arg,
-      (* TODO: what is the semantics of node application? *)
-    Lsem_equation env (EqApp x f arg).
-
-Definition Lsem_equations (env : Lvenv) (eqs : list equation) : Prop :=
-  List.Forall (Lsem_equation env) eqs.
-
-Inductive Lsem_node (env : Lvenv) : node -> Prop :=
-| Lnode:
-    forall name input output eqs env' s_input s_output,
-      PositiveMap.add input.(v_name) s_input 
-       (PositiveMap.add output.(v_name) s_output env) = env' ->
-      Lsem_equations env' eqs ->
-      Lsem_node env (mk_node name input output eqs).
+      (exists H' vi vo, (* local context (history), input values and output values *)
+          sem_laexp H arg vi (* arg evaluate to vi *)
+       /\ sem_lexp H (Evar x) vo (* x evaluates to vo *)
+       /\ sem_lexp H' (Evar input.(v_name)) vi (* in the local context, input evaluates to vi *)
+       /\ sem_lexp H' (Evar output.(v_name)) vo  (* in the local context, output evaluates to vo *)
+       /\ List.Forall (sem_equation G H') eqs) (* in the local context, the equations have correct semantics *)
+      -> sem_equation G H (EqApp x f arg)
+  | SEqFby : forall H x v cae,
+      (exists cl, sem_caexp H cae cl /\ sem_lexp H (Evar x) (fby v cl)) ->
+      sem_equation G H (EqFby x v cae).
