Common.v
@@ -10,3 +10,6 @@ Definition ident := positive.
 Inductive const : Set :=
 | Cint : BinInt.Z -> const
 | Cbool : bool -> const.
+
+Coercion Cint : BinInt.Z >-> const.
+Coercion Cbool : bool >-> const.
